**Tags:** #Theorem #Analysis/Differentiation #Course/FPM 

> [!Theorem]+ Thm: [[Taylor Series]]
> Suppose that $f:(a,b)\to\R$ is infinitely differentiable and let $x_{0}\in (a,b)$. Fix $x$ in $(a,b)$. For every positive integer $N$ we have
> $$f(x)=\sum_{k=0}^{N} \frac{f^{(k)}(x_{0})}{k!}(x-x_{0})^{k} + R_{N}(x)$$
> We can think of
> $$\sum_{k=0}^{N} \frac{f^{(k)}(x_{0})}{k!}(x-x_{0})^{k}$$
> as the $N$th partial sum of the series
> $$\sum_{k=0}^{\infty} \frac{f^{(k)}(x_{0})}{k!}(x-x_{0})^{k}$$
> (taylor series of $f$ with center $x_{0}$)
> With $x$ still fixed, write
> $$\sum_{k=0}^{N} \frac{f^{(k)}(x_{0})}{k!}(x-x_{0})^{k}=f(x)-R_{N}(x)$$

^0255ee


